

We begin with a 3 point rank-2 integral

$$\int_l \frac{l^{\mu_1} l^{\mu_2}}{[l^2 - m^2][(l + k_1)^2 - m^2][(l + k_2)^2 - m^2]} \quad (1)$$

Performing Feynman parametrization

$$\int_0^1 dxdy \int_l \frac{l^{\mu_1} l^{\mu_2}}{[l^2 + 2l.k_1x + 2l.k_2y - m^2]^3} \quad (2)$$

Adding $k_1.k_1x^2 = 0$, $k_2.k_2y^2 = 0$ and $k_1.k_2xy - k_1.k_2xy = 0$ we have:

$$= \int_0^1 dxdy \int_l \frac{l^{\mu_1} l^{\mu_2}}{[(l + k_1x + k_2y)^2 - k_1.k_2xy - m^2]^3} \quad (3)$$

$$= \int_0^1 dxdy \int_l \frac{(l - 2k_1x - 2k_2y)^{\mu_1} (l - 2k_1x - 2k_2y)^{\mu_2}}{[l^2 - 2k_1.k_2xy - m^2]^3} \quad (4)$$